Linglib.lean
@@ -99,7 +99,6 @@ import Linglib.Core.Computability.Variety.Equations
 import Linglib.Core.Computability.Variety.Langs
 import Linglib.Core.Computability.Variety.OmegaEquations
 import Linglib.Core.Computability.Variety.SemigroupLangs
-import Linglib.Core.Computability.WordModel
 import Linglib.Core.Data.Fin.Tuple.Basic
 import Linglib.Core.Data.Fintype.Sets
 import Linglib.Core.Data.Fintype.Transfer
